theories/degree.v
@@ -1,0 +1,82 @@
+Require Export imports.
+
+Definition DBasis := nat -> nat.
+
+Fixpoint degree (Ξ : DBasis) a :=
+  match a with
+  | VarTm i => Ξ i
+  | ISort Star => 2
+  | ISort Kind => 3
+  | Abs A a => degree (degree Ξ A - 1 .: Ξ) a
+  | Pi A B => degree (degree Ξ A - 1 .: Ξ) B
+  | App a b => degree Ξ a
+  end.
+
+Fixpoint b2d Γ :=
+  match Γ with
+  | nil => ids
+  | A :: Γ =>
+      degree (b2d Γ) A - 1 .: b2d Γ
+  end.
+
+Definition ξ_ok ξ (Ξ0 Ξ1 : DBasis) := forall i, Ξ0 i = Ξ1 (ξ i).
+
+Lemma ξ_ok_up ξ Ξ0 Ξ1 i : ξ_ok ξ Ξ0 Ξ1 ->
+                            ξ_ok (upRen_Term_Term ξ) (i .: Ξ0) (i .: Ξ1).
+Proof.
+  move => h.
+  case => //=.
+Qed.
+
+Lemma renaming Ξ a : forall ξ Ξ', ξ_ok ξ Ξ Ξ' -> degree Ξ a = degree Ξ' a⟨ξ⟩.
+Proof.
+  elim : a Ξ=>//=; hauto lq:on use:ξ_ok_up.
+Qed.
+
+Definition ρ_ok ρ (Ξ0 Ξ1 : DBasis) :=
+  forall i, degree Ξ1 (ρ i) = Ξ0 i.
+
+Lemma ρ_ext ρ (Ξ0 Ξ1 : DBasis) a i :
+  ρ_ok ρ Ξ0 Ξ1 ->
+  degree Ξ1 a = i ->
+  ρ_ok (a .: ρ) (i .: Ξ0) Ξ1.
+Proof.
+  move => hρ.
+  rewrite /ρ_ok => h.
+  case => //=.
+Qed.
+
+Lemma ρ_ξ_comp ρ ξ Ξ0 Ξ1 Ξ2 :
+  ρ_ok ρ Ξ0 Ξ1 ->
+  ξ_ok ξ Ξ1 Ξ2 ->
+  ρ_ok (ρ >> ren_Term ξ) Ξ0 Ξ2.
+Proof.
+  rewrite /ρ_ok /ξ_ok => hρ hξ i.
+  have -> : (ρ >> ren_Term  ξ ) i = (ρ i)⟨ ξ ⟩ by asimpl.
+  rewrite -(renaming Ξ1) => //=.
+Qed.
+
+Lemma ρ_up ρ Ξ0 Ξ1 i :
+  ρ_ok ρ Ξ0 Ξ1 ->
+  ρ_ok (up_Term_Term ρ) (i .: Ξ0) (i .: Ξ1).
+Proof.
+  move => hρ.
+  rewrite /up_Term_Term.
+  apply ρ_ext => //=.
+  apply : ρ_ξ_comp; eauto.
+  rewrite /ξ_ok. case => //=.
+Qed.
+
+Lemma morphing Ξ a : forall ρ Ξ', ρ_ok ρ Ξ Ξ' -> degree Ξ a = degree Ξ' a[ρ].
+Proof.
+  elim : a Ξ => //=; hauto lq:on use:ρ_up.
+Qed.
+
+Lemma ρ_id Ξ :
+  ρ_ok ids Ξ Ξ.
+Proof. by rewrite /ρ_ok. Qed.
+
+Lemma subst_one Ξ a b i :
+  degree Ξ b = i ->
+  degree (i .: Ξ) a = degree Ξ a[b…].
+Proof. eauto using morphing, ρ_ext, ρ_id. Qed.
